Refinery/Term/Extrinsic/Semantics/Subst/Coherent.lean
@@ -1,0 +1,27 @@
+import Refinery.Term.Extrinsic.Semantics.Subst
+import Refinery.Term.Extrinsic.Semantics.Minimal
+
+namespace Refinery
+
+open CategoryTheory
+
+open MonoidalCategory' PremonoidalCategory DistributiveCategory ChosenFiniteCoproducts
+      HasQuant HasCommRel EffectfulCategory BraidedCategory' SymmetricCategory'
+
+open scoped MonoidalCategory
+
+namespace Term
+
+variable {φ : Type _} {α : outParam (Type _)} {ε : outParam (Type _)} [S : Signature φ α ε]
+         {C : Type _} [Category C] [PremonoidalCategory C] [CC : ChosenFiniteCoproducts C]
+        [SymmetricCategory' C] [Iterate C] [E : Elgot2 C ε] [M : Model φ α ε C]
+
+theorem Deriv.den_subst_pos' {eσ ea : ε} (he : eσ ⇀ ea)
+  {Γ Δ : Ctx? α} (σ : SubstDS φ Γ Δ) [hσ : σ.Pos eσ] {A : Ty α} {a : Term φ (Ty α)}
+  (D : Δ ⊢ a : A) [ha : a.HasEff ea] (Dσ : Γ ⊢ a.subst σ : A) : σ.den ≫ D.den ↠ Dσ.den (C := C)
+  := by convert D.den_subst_pos he σ using 1; apply Deriv.coherence
+
+theorem Deriv.den_subst_neg' {eσ ea : ε} (he : eσ ↽ ea)
+  {Γ Δ : Ctx? α} (σ : SubstDS φ Γ Δ) [hσ : σ.Neg eσ] {A : Ty α} {a : Term φ (Ty α)}
+  (D : Δ ⊢ a : A) [ha : a.HasEff ea] (Dσ : Γ ⊢ a.subst σ : A) : σ.den ≫ D.den ↞ Dσ.den (C := C)
+  := by convert D.den_subst_neg he σ using 1; apply Deriv.coherence
