Refinery/Term/Syntax/FreeVar.lean
@@ -1,0 +1,1 @@
+--TODO: utilities for counting free variables, substituting and renaming up to free variables
